### Lec 2/15

#### Map Pattern 

```haskell
{-do sth to each elem in the list-}
squares [] = []
squares (x:xs) = (x*x) : squares xs

map f [] = []
map f (x:xs) = f x : map f xs

map :: (a -> b) -> [a] -> [b]
quiz = map (\(x, y) -> x + y) [(1, 2)]

addAdjacent  :: [Int] -> [Int]
```

#### fold-right pattern 

```haskell
--pattern 
{-
	foo op b (x:xs)
	
	   operand -> base case -> list of data
-}

Op -> Type_b -> [Type_a] -> Type_b
(\Type_a Type_b -> Type_b) -> Type_b -> [Type_a] -> Type_b
=> (a -> b -> b) -> b -> [a] -> b

foldr f b [] = b
foldr f b (x:xs) = x `f` (foldr op b xs)

-- recurse on tail
-- combine result with head using some binary operation 

concatList :: [String] -> String 
concatList = foo (++) "" 

concatList ["this", "is", "a", "test"]

{-
foldr op b (x1, x2, x3, x4, x5)
=> op x1 (foldr op b (x2, x3, x4, x5))

=> x1 `op` x2 `op` x3 `op` x4 `op` x5 `op` b
-}

quiz = foldr (\x v -> x : v) [] [1, 2, 3]

```

![Screen Shot 2022-02-23 at 15.16.20](/Users/heyilang/Library/Application Support/typora-user-images/Screen Shot 2022-02-23 at 15.16.20.png)

#### Fold-Left

Tail Recursive Fold

```haskell
foldr f b [] = b
foldr f b (x:xs) = x `f` (foldr op b xs)

sumTR :: [Int] -> Int
sumTR xs = loop 0 xs 
	where 
		loop n [] = n
		loop n [x:xs] = loop (n+x) xs
		
sumTR' = loop (\res x -> res + x) 0 xs 
-- AKA sumTR' = loop (+) 0 xs

loop op res [] = res
loop op res (x:xs) = loop (op res x) xs
```





#### 

